![image](https://github.com/ManchanTime/TrashBoys/assets/127479677/1457d46f-dba4-4a2c-a3f1-a99d3bd8928f)

해 구해기

ax + by = c
dx + ey = f

==> aex + bey = ce
    bdx + bey = fb
    => (ae-bd)x = ce-fb => x = (ce-fb)/(ae-bd)로 나타낼 수 있고 이 때 ae-bd가 0이라면 x의 해는 0으로 볼 수 있음!!
    같은 방식으로 y를 구하면
    adx + bdy = cd
    adx + aey = af
    => (bd-ae)y = (cd-af) => y = (cd-af)/(bd-ae) => bd-ae가 0 이면 y의 해는 0

  ![image](https://github.com/ManchanTime/TrashBoys/assets/127479677/c3abfb26-e525-4baf-9d92-cfdb5bc8c6fe)
